adding description to configured invariant

Network_Security_Policy_Verification/Examples/Impl_List_Playground_ChairNetwork.thy
@@ -23,7 +23,7 @@ subsection{*Our security requirements*}
           node_properties = [''FilesSrv'' \<mapsto> \<lparr> privacy_level = 1, trusted = False \<rparr>,
                              ''Employees'' \<mapsto> \<lparr> privacy_level = 0, trusted = True \<rparr>,
                              ''EReachable'' \<mapsto> \<lparr> privacy_level = 0, trusted = True \<rparr>]
-          \<rparr>"
+          \<rparr> ''confidential data''"
 
 
   (*
@@ -47,28 +47,28 @@ subsection{*Our security requirements*}
                              ''Employees'' \<mapsto> Care,
                              ''EReachable'' \<mapsto> Care,
                              ''Students'' \<mapsto> Care]
-          \<rparr>"
+          \<rparr> ''printing ACL''"
 
   subsubsection{* Printers are information sinks *}
     definition "PrintingSink \<equiv> new_configured_list_SecurityInvariant SINVAR_LIB_Sink \<lparr> 
           node_properties = [''PrinterColor'' \<mapsto> Sink,
                              ''PrinterBW'' \<mapsto> Sink]
-          \<rparr>"
+          \<rparr> ''printing sink''"
 
 
 
   subsubsection{*Students may access each other but are not accessible from the outside*}
     definition "StudentSubnet \<equiv> new_configured_list_SecurityInvariant SINVAR_LIB_SubnetsInGW \<lparr> 
           node_properties = [''Students'' \<mapsto> Member, ''Employees'' \<mapsto> Member, ''EReachable'' \<mapsto> InboundGateway]
-          \<rparr>"
+          \<rparr> ''student subnet''"
 
 
   subsubsection{* The files server is only accessibly by employees*}
-    definition "FilesSrcACL \<equiv> new_configured_list_SecurityInvariant SINVAR_LIB_CommunicationPartners \<lparr> 
+    definition "FilesSrvACL \<equiv> new_configured_list_SecurityInvariant SINVAR_LIB_CommunicationPartners \<lparr> 
           node_properties = [''FilesSrv'' \<mapsto> Master [''Employees'', ''EReachable''],
                              ''Employees'' \<mapsto> Care,
                              ''EReachable'' \<mapsto> Care]
-          \<rparr>"
+          \<rparr> ''file srv acl''"
 
 
   subsubsection{*emplyees are reachable from the Internet*}
@@ -78,9 +78,9 @@ lemma "implc_sinvar ConfidentialChairData ChairNetwork_empty" by eval
 lemma "implc_sinvar PrintingACL ChairNetwork_empty" by eval
 lemma "implc_sinvar PrintingSink ChairNetwork_empty" by eval
 lemma "implc_sinvar StudentSubnet ChairNetwork_empty" by eval
-lemma "implc_sinvar FilesSrcACL ChairNetwork_empty" by eval
+lemma "implc_sinvar FilesSrvACL ChairNetwork_empty" by eval
 
-definition "ChairSecurityRequirements = [ConfidentialChairData, PrintingACL, PrintingSink, StudentSubnet, FilesSrcACL]"
+definition "ChairSecurityRequirements = [ConfidentialChairData, PrintingACL, PrintingSink, StudentSubnet, FilesSrvACL]"
 
 value "implc_get_offending_flows ChairSecurityRequirements ChairNetwork_empty"
 value "generate_valid_topology ChairSecurityRequirements ChairNetwork_empty"
